TotalUtil.thy
@@ -126,4 +126,230 @@ lemma prat_positive_transfer:
   apply transfer
   by simp
 
+subsection \<open>Disjoint lists\<close>
+
+definition disjoint_list :: " ('a set) list \<Rightarrow> bool"
+  where "disjoint_list xs = (\<forall>i j. 0 \<le> i \<and> i < length xs \<and> 0 \<le> j \<and> j < length xs \<and> i \<noteq> j \<longrightarrow> disjnt (xs ! i) (xs ! j))"
+
+lemma disjoint_list_app_disj:
+  assumes "disjoint_list (xs@ys)" and
+          "x \<in> set xs" and
+          "y \<in> set ys"
+        shows "disjnt x y"
+proof -
+  from \<open>x \<in> set xs\<close> obtain i where "0 \<le> i" and "i < length xs" and "x = xs ! i"
+    by (metis bot_nat_0.extremum in_set_conv_nth)
+  hence xElem: "x = (xs@ys) ! i"
+    using List.nth_append
+    by metis
+
+  from \<open>y \<in> set ys\<close> obtain j where "0 \<le> j" and "j < length ys" and "y = ys ! j"
+    by (metis bot_nat_0.extremum in_set_conv_nth)
+  hence "y = (xs@ys) ! (length xs + j)"
+    using List.nth_append
+    by auto
+
+  with xElem \<open>0 \<le> i\<close> \<open>i < length xs\<close> \<open>0 \<le> j\<close> \<open>j < length ys\<close> show ?thesis
+    using assms
+    unfolding disjoint_list_def
+    by (simp add: add.commute)
+qed
+
+lemma disjoint_list_add:
+  assumes Disj: "disjoint_list (xs@(M#ys))" and
+          Fresh: "\<forall>A \<in> set (xs@(M#ys)). m \<notin> A" \<comment>\<open>Can weaken this s.t. m can be included in M\<close>
+        shows "disjoint_list (xs@((M \<union> {m})#ys))"
+  unfolding disjoint_list_def
+proof (rule allI | rule impI)+
+  fix i j
+  assume Bounds: "0 \<le> i \<and> i < length (xs @ (M \<union> {m}) # ys) \<and> 0 \<le> j \<and> j < length (xs @ (M \<union> {m}) # ys) \<and> i \<noteq> j"
+  hence "i \<noteq> j"
+    by simp
+
+  have DisjXsM: "\<And>x. x \<in> set xs \<Longrightarrow> disjnt x (M \<union> {m})"
+    using assms disjoint_list_app_disj
+    by fastforce
+
+  have DisjXsYs: "\<And>x y. x \<in> set xs \<Longrightarrow> y \<in> set ys \<Longrightarrow> disjnt x y"
+    using Disj disjoint_list_app_disj
+    by fastforce
+
+  have DisjYsM: "\<And>y. y \<in> set ys \<Longrightarrow> disjnt (M \<union> {m}) y"
+  proof -
+    fix y
+    assume "y \<in> set ys"
+    from Disj have "disjoint_list ((xs@[M])@ys)" 
+      by simp
+    hence "disjnt M y"
+      using \<open>y \<in> _\<close> disjoint_list_app_disj
+      by fastforce
+    thus "disjnt (M \<union> {m}) y"
+      using Fresh \<open>y \<in> set ys\<close> by fastforce
+  qed  
+
+  have ElemYsAux: "\<And>j. length xs < j \<Longrightarrow> j < length (xs @ (M \<union> {m}) # ys) \<Longrightarrow> (xs @ ((M \<union> {m}) # ys)) ! j \<in> set ys"
+  proof -
+    fix j
+    assume "length xs < j" and "j < length (xs @ (M \<union> {m}) # ys)"
+
+    hence "j \<ge> length (xs @ [M \<union> {m}])"
+            by simp 
+
+   let ?b = "(xs @ ((M \<union> {m}) # ys)) ! j"
+          
+    have Eq: "(xs @ (M \<union> {m}) # ys) = ((xs @ [M \<union> {m}]) @ ys)"
+      by simp
+ 
+    from \<open>j \<ge> length (xs @ [M \<union> {m}])\<close> \<open>j < length (xs @ (M \<union> {m}) # ys)\<close> obtain j' where
+       "?b = ys ! j'" and "j' = j - (length (xs @ [M \<union> {m}]))"
+      using Eq List.nth_append[where ?ys=ys] 
+      by (metis linorder_not_less)            
+      
+    thus "?b \<in> set ys"
+      using \<open>j \<ge> length (xs @ [M \<union> {m}])\<close> and \<open>j < length (xs @ (M \<union> {m}) # ys)\<close>
+      by simp
+  qed
+
+
+  have Aux: "\<And>i j. 0 \<le> i \<and> i < length (xs @ (M \<union> {m}) # ys) \<and> 0 \<le> j \<and> j < length (xs @ (M \<union> {m}) # ys) \<and> i \<noteq> j \<Longrightarrow>
+               i < length xs  \<Longrightarrow> disjnt ((xs @ (M \<union> {m}) # ys) ! i) ((xs @ (M \<union> {m}) # ys) ! j)"
+  proof -
+    fix i j
+    assume Bounds: "0 \<le> i \<and> i < length (xs @ (M \<union> {m}) # ys) \<and> 0 \<le> j \<and> j < length (xs @ (M \<union> {m}) # ys) \<and> i \<noteq> j"
+    hence "i \<noteq> j"
+      by simp
+    assume A: "i < length xs"
+    show "disjnt ((xs @ (M \<union> {m}) # ys) ! i) ((xs @ (M \<union> {m}) # ys) ! j)" (is "disjnt ?a ?b")
+    proof -
+      from A
+      have "?a \<in> set xs"
+        using List.nth_append
+        by (metis nth_mem)
+
+      with A have "?a = (xs @ M # ys) ! i"
+        using List.nth_append
+        by metis
+
+    then show ?thesis
+    proof (cases "0 \<le> j \<and> j < length xs")
+      case True 
+        hence "?b \<in> set xs"
+        using List.nth_append
+        by (metis nth_mem)
+
+      with True have "?b = (xs @ M # ys) ! j"
+        using List.nth_append
+        by metis
+      with \<open>?a = _\<close> 
+      show ?thesis
+        using Disj A Bounds \<open>0 \<le> j \<and> j < length xs\<close> \<open>i \<noteq> j\<close>
+        unfolding disjoint_list_def
+        by simp                
+    next
+      case False
+        with Bounds have "length xs \<le> j" and "j < length (xs @ (M \<union> {m}) # ys)"
+          by auto
+
+        show ?thesis
+        proof (cases "j = length xs")
+          case True
+          hence "?b = (M \<union> {m})"
+            by simp
+          then show ?thesis 
+            using DisjXsM \<open>?a \<in> set xs\<close>
+            by simp
+        next
+          case False
+          hence "?b \<in> set ys"
+            using ElemYsAux \<open>j < length (xs @ (M \<union> {m}) # ys)\<close> \<open>length xs \<le> j\<close> by fastforce  
+
+          with \<open>?a \<in> set xs\<close>  show ?thesis
+            using DisjXsYs
+            by simp
+        qed
+      qed
+    qed
+  qed
+
+  show "disjnt ((xs @ (M \<union> {m}) # ys) ! i) ((xs @ (M \<union> {m}) # ys) ! j)" (is "disjnt ?a ?b")
+  proof (cases "i < length xs")
+    case True
+    then show ?thesis using Aux[OF Bounds]
+      by simp      
+  next
+    case False
+    hence "i \<ge> length xs"
+      by simp
+
+    show ?thesis 
+    proof (cases "j < length xs")
+      case True
+      \<comment>\<open>We have already shown the symmetric case\<close>
+      then show ?thesis 
+        using Aux Bounds disjnt_sym
+        by blast
+    next
+      case False
+      hence "j \<ge> length xs"
+        by simp
+      \<comment>\<open>Now we prove the case where \<^term>\<open>i = length xs\<close> and thus \<^term>\<open>j > length xs\<close>. We can then prove
+        the case where  \<^term>\<open>i > length xs\<close> and \<^term>\<open>j = length xs\<close> by symmetry\<close>
+
+      have Aux2: "\<And>i j. i = length xs \<Longrightarrow> j > length xs \<Longrightarrow> j < length (xs @ (M \<union> {m}) # ys) \<Longrightarrow> i \<noteq> j \<Longrightarrow>
+                disjnt ((xs @ (M \<union> {m}) # ys) ! i) ((xs @ (M \<union> {m}) # ys) ! j)"
+      proof -
+        fix i j
+        assume "i = length xs" and "length xs < j" and "j < length (xs @ (M \<union> {m}) # ys)" and "i \<noteq> j"
+        show "disjnt ((xs @ (M \<union> {m}) # ys) ! i) ((xs @ (M \<union> {m}) # ys) ! j)" (is "disjnt ?a ?b")
+        proof -
+          from \<open>i = length xs\<close> have "?a = M \<union> {m}"
+            by simp
+
+          have "?b \<in> set ys"
+            using ElemYsAux \<open>j < length (xs @ (M \<union> {m}) # ys)\<close> \<open>length xs < j\<close> 
+            by blast
+
+          thus ?thesis
+            using \<open>?a = _\<close> DisjYsM
+            by simp
+        qed
+      qed
+
+      show ?thesis
+      proof (cases "i = length xs")
+        case True
+        thus ?thesis
+          using Aux2 \<open>j \<ge> length xs\<close>  Bounds
+          by auto                              
+      next
+        case False
+        show ?thesis 
+        proof (cases "j = length xs")
+          case True
+          then show ?thesis using Aux2 \<open>i \<ge> length xs\<close> Bounds
+            by (metis disjnt_sym order_le_neq_trans)
+        next
+          case False
+          have Eq: "length (xs @ M # ys) = length (xs @ (M \<union> {m}) # ys)" 
+            by simp
+
+          have "disjnt ((xs @ M # ys) ! i) ((xs @ M # ys) ! j)"
+            using Disj \<open>i \<noteq> j\<close> \<open>i \<ge> length xs\<close> \<open>j \<ge> length xs\<close>
+            unfolding disjoint_list_def 
+            apply (simp only: Eq)
+            using Bounds by blast
+            
+
+          moreover have "?a = (xs @ M # ys) ! i" and "?b = (xs @ M # ys) ! j"                    
+             apply (metis \<open>i \<noteq> length xs\<close> list_update_length nth_list_update_neq)
+            by (metis False list_update_length nth_list_update_neq)             
+          ultimately show ?thesis
+            by argo                        
+        qed
+      qed
+    qed
+  qed
+qed
+
+
 end
